theories/typing/own.v
@@ -268,7 +268,7 @@ Section typing.
       have ->: (subst x xv (x <- p;; e))%E = (xv <- p;; subst x xv e)%E.
       { rewrite /subst /=. repeat f_equal;
         [by rewrite bool_decide_true|eapply is_closed_subst=>//; set_solver]. }
-      iApply type_assign; [|solve_typing|by eapply write_own|done|done].
+      iApply type_assign; [|solve_typing|by eapply write_own|done].
       apply subst_is_closed; [|done]. apply is_closed_of_val. }
     by move=>/= [??]??.
   Qed.
@@ -293,7 +293,7 @@ Section typing.
         - eapply (is_closed_subst []); [apply is_closed_of_val|set_solver].
         - by rewrite bool_decide_true.
         - eapply is_closed_subst; [done|set_solver]. } rewrite Nat2Z.id.
-      iApply type_memcpy; [|solve_typing| |solve_typing|done|done|done].
+      iApply type_memcpy; [|solve_typing| |done|done|done].
       { apply subst_is_closed; [|done]. apply is_closed_of_val. }
       by apply write_own. } by move=>/= [??]??.
   Qed.
